src/prop/SemiReachable.v
@@ -1,0 +1,666 @@
+Require Import Omega.
+Require Import Bool.
+Require Import RelationClasses.
+
+From sflib Require Import sflib.
+From Paco Require Import paco.
+
+From PromisingLib Require Import Axioms.
+From PromisingLib Require Import Basic.
+From PromisingLib Require Import DataStructure.
+From PromisingLib Require Import DenseOrder.
+From PromisingLib Require Import Language.
+From PromisingLib Require Import Loc.
+
+Require Import Event.
+Require Import Time.
+Require Import View.
+Require Import Cell.
+Require Import Memory.
+Require Import TView.
+Require Import Local.
+Require Import Thread.
+Require Import Configuration.
+Require Import Trace.
+Require Import Behavior.
+Require Import Single.
+Require Import Mapping.
+
+Set Implicit Arguments.
+
+Module SemiReachable.
+  Section REACHABLE.
+
+    Variable (c0: Configuration.t).
+
+    Hypothesis CONFIG_CONSISTENT: forall tid lang st lc
+                                         (TID: IdentMap.find tid c0.(Configuration.threads) = Some (existT _ lang st, lc)),
+        Local.promise_consistent lc.
+    Hypothesis CONFIG_WF: Configuration.wf c0.
+
+    Section TID.
+
+      Variable (tid: Ident.t).
+
+      Inductive semi_reachable lang (th: Thread.t lang): Prop :=
+      | semi_reachable_intro
+          c1 st1 lc1
+          (STEPS: rtc SConfiguration.all_machine_step c0 c1)
+          (TID: IdentMap.find tid c1.(Configuration.threads) = Some (existT _ lang st1, lc1))
+          (TSTEPS: rtc (@Thread.all_step _) (Thread.mk _ st1 lc1 c1.(Configuration.sc) c1.(Configuration.memory)) th)
+          (CONSISTENT: Local.promise_consistent th.(Thread.local))
+      .
+      Hint Constructors semi_reachable.
+
+      Inductive semi_reachable_state
+                (lang: language) (st: @Language.state _ lang): Prop :=
+      | semi_reachable_stateintro
+          lc sc mem
+          (REACHABLE: semi_reachable (Thread.mk _ st lc sc mem))
+        :
+          semi_reachable_state _ st
+      .
+      Hint Constructors semi_reachable_state.
+
+      Inductive step lang: forall (pf: bool) (e: ThreadEvent.t) (th0 th1: Thread.t lang), Prop :=
+      | step_intro
+          pf e th0 th1
+          (STEP: Thread.step pf e th0 th1)
+          (REACHABLE: semi_reachable_state lang th1.(Thread.state))
+        :
+          step pf e th0 th1
+      .
+      Hint Constructors step.
+
+      Inductive opt_step lang: forall (e:ThreadEvent.t) (e1 e2:Thread.t lang), Prop :=
+      | step_none
+          e:
+          opt_step ThreadEvent.silent e e
+      | step_some
+          pf e e1 e2
+          (STEP: step pf e e1 e2):
+          opt_step e e1 e2
+      .
+      Hint Constructors opt_step.
+
+      Inductive step_allpf lang (e:ThreadEvent.t) (e1 e2:Thread.t lang): Prop :=
+      | step_nopf_intro
+          pf
+          (STEP: step pf e e1 e2)
+      .
+      Hint Constructors step_allpf.
+
+      Definition tau_step lang := tau (@step_allpf lang).
+
+      Inductive reserve_step lang (e1 e2:Thread.t lang): Prop :=
+      | reserve_step_intro
+          pf loc from to
+          (STEP: step pf (ThreadEvent.promise loc from to Message.reserve Memory.op_kind_add) e1 e2)
+      .
+      Hint Constructors reserve_step.
+
+      Inductive cancel_step lang (e1 e2:Thread.t lang): Prop :=
+      | cancel_step_intro
+          pf loc from to
+          (STEP: step pf (ThreadEvent.promise loc from to Message.reserve Memory.op_kind_cancel) e1 e2)
+      .
+      Hint Constructors cancel_step.
+
+      Lemma step_reachable lang pf e (th0 th1: Thread.t lang)
+            (STEP: Thread.step pf e th0 th1)
+            (CONSISTENT: Local.promise_consistent th1.(Thread.local))
+            (REACHABLE: semi_reachable th0)
+        :
+          (<<STEP: step pf e th0 th1>>) /\
+          (<<REACHABLE: semi_reachable th1>>).
+      Proof.
+        inv REACHABLE.
+        assert (REACHABLE0: semi_reachable th1).
+        { econs; eauto. etrans; eauto. econs 2; [|refl]. econs; eauto. econs; eauto. }
+        splits; auto. econs; eauto. destruct th1. econs; eauto.
+      Qed.
+
+      Lemma opt_step_reachable lang e (th0 th1: Thread.t lang)
+            (STEP: Thread.opt_step e th0 th1)
+            (CONSISTENT: Local.promise_consistent th1.(Thread.local))
+            (REACHABLE: semi_reachable th0)
+        :
+          (<<STEP: opt_step e th0 th1>>) /\
+          (<<REACHABLE: semi_reachable th1>>).
+      Proof.
+        inv STEP.
+        - splits; auto.
+        - eapply step_reachable in STEP0; eauto. des. splits; eauto.
+      Qed.
+
+      Lemma tau_steps_reachable lang (th0 th1: Thread.t lang)
+            (STEPS: rtc (@Thread.tau_step _) th0 th1)
+            (LOCAL: Local.wf th0.(Thread.local) th0.(Thread.memory))
+            (MEMORY: Memory.closed th0.(Thread.memory))
+            (SC: Memory.closed_timemap th0.(Thread.sc) th0.(Thread.memory))
+            (CONSISTENT: Local.promise_consistent th1.(Thread.local))
+            (REACHABLE: semi_reachable th0)
+        :
+          (<<STEP: rtc (@tau_step _) th0 th1>>) /\
+          (<<REACHABLE: semi_reachable th1>>).
+      Proof.
+        revert LOCAL MEMORY SC CONSISTENT REACHABLE. induction STEPS; eauto. i.
+        inv H. inv TSTEP. exploit Thread.step_future; eauto. i. des.
+        hexploit PromiseConsistent.rtc_tau_step_promise_consistent; eauto. i.
+        hexploit step_reachable; eauto. i. des.
+        hexploit IHSTEPS; eauto. i. des. splits; eauto.
+        econs; eauto. econs; eauto.
+      Qed.
+
+      Lemma reserve_steps_reachable lang (th0 th1: Thread.t lang)
+            (STEPS: rtc (@Thread.reserve_step _) th0 th1)
+            (LOCAL: Local.wf th0.(Thread.local) th0.(Thread.memory))
+            (MEMORY: Memory.closed th0.(Thread.memory))
+            (SC: Memory.closed_timemap th0.(Thread.sc) th0.(Thread.memory))
+            (CONSISTENT: Local.promise_consistent th1.(Thread.local))
+            (REACHABLE: semi_reachable th0)
+        :
+          (<<STEP: rtc (@reserve_step _) th0 th1>>) /\
+          (<<REACHABLE: semi_reachable th1>>).
+      Proof.
+        revert LOCAL MEMORY SC CONSISTENT REACHABLE. induction STEPS; eauto. i.
+        inv H. exploit Thread.step_future; eauto. i. des.
+        hexploit PromiseConsistent.rtc_reserve_step_promise_consistent; eauto. i.
+        hexploit step_reachable; eauto. i. des.
+        hexploit IHSTEPS; eauto. i. des. splits; eauto.
+      Qed.
+
+      Lemma cancel_steps_reachable lang (th0 th1: Thread.t lang)
+            (STEPS: rtc (@Thread.cancel_step _) th0 th1)
+            (LOCAL: Local.wf th0.(Thread.local) th0.(Thread.memory))
+            (MEMORY: Memory.closed th0.(Thread.memory))
+            (SC: Memory.closed_timemap th0.(Thread.sc) th0.(Thread.memory))
+            (CONSISTENT: Local.promise_consistent th1.(Thread.local))
+            (REACHABLE: semi_reachable th0)
+        :
+          (<<STEP: rtc (@cancel_step _) th0 th1>>) /\
+          (<<REACHABLE: semi_reachable th1>>).
+      Proof.
+        revert LOCAL MEMORY SC CONSISTENT REACHABLE. induction STEPS; eauto. i.
+        inv H. exploit Thread.step_future; eauto. i. des.
+        hexploit PromiseConsistent.rtc_cancel_step_promise_consistent; eauto. i.
+        hexploit step_reachable; eauto. i. des.
+        hexploit IHSTEPS; eauto. i. des. splits; eauto.
+      Qed.
+
+      Definition consistent lang (e1:Thread.t lang): Prop :=
+        forall mem1 sc1
+               (CAP: Memory.cap e1.(Thread.memory) mem1)
+               (SC_MAX: Memory.max_concrete_timemap mem1 sc1),
+          (exists e2 e3,
+              (<<STEPS: rtc (@tau_step lang) (Thread.mk _ e1.(Thread.state) e1.(Thread.local) sc1 mem1) e2>>) /\
+              (<<FAILURE: step true ThreadEvent.failure e2 e3 >>)) \/
+          (exists e2,
+              (<<STEPS: rtc (@tau_step lang) (Thread.mk _ e1.(Thread.state) e1.(Thread.local) sc1 mem1) e2>>) /\
+              (<<PROMISES: e2.(Thread.local).(Local.promises) = Memory.bot>>))
+      .
+
+      Inductive configuration_step:
+        forall (e:ThreadEvent.t) (tid:Ident.t) (c1 c2:Configuration.t), Prop :=
+      | configuration_step_intro
+          e tid c1 lang st1 lc1 e2 e3 st4 lc4 sc4 memory4
+          (TID: IdentMap.find tid c1.(Configuration.threads) = Some (existT _ lang st1, lc1))
+          (CANCELS: rtc (@cancel_step _) (Thread.mk _ st1 lc1 c1.(Configuration.sc) c1.(Configuration.memory)) e2)
+          (STEP: opt_step e e2 e3)
+          (RESERVES: rtc (@reserve_step _) e3 (Thread.mk _ st4 lc4 sc4 memory4))
+          (CONSISTENT: e <> ThreadEvent.failure -> consistent (Thread.mk _ st4 lc4 sc4 memory4)):
+          configuration_step e tid c1 (Configuration.mk (IdentMap.add tid (existT _ _ st4, lc4) c1.(Configuration.threads)) sc4 memory4)
+      .
+      Hint Constructors configuration_step.
+
+      Lemma step_map_reachable lang pf e (th0 th1 fth0: Thread.t lang)
+            (STEP: Thread.step pf e th0 th1)
+            (THREAD: thread_map ident_map th0 fth0)
+            (CONSISTENT: Local.promise_consistent th1.(Thread.local))
+            (REACHABLE: semi_reachable fth0)
+            (LOCAL: Local.wf th0.(Thread.local) th0.(Thread.memory))
+            (MEMORY: Memory.closed th0.(Thread.memory))
+            (SC: Memory.closed_timemap th0.(Thread.sc) th0.(Thread.memory))
+            (FLOCAL: Local.wf fth0.(Thread.local) fth0.(Thread.memory))
+            (FMEMORY: Memory.closed fth0.(Thread.memory))
+            (FSC: Memory.closed_timemap fth0.(Thread.sc) fth0.(Thread.memory))
+        :
+          exists fpf fe fth1,
+            (<<STEP: Thread.step fpf fe fth0 fth1>>) /\
+            (<<EVENT: tevent_map ident_map fe e>>) /\
+            (<<THREAD: thread_map ident_map th1 fth1>>) /\
+            (<<REACHABLE: semi_reachable fth1>>) /\
+            (<<STEP: step pf e th0 th1>>)
+      .
+      Proof.
+        splits; auto.
+        inv THREAD. destruct th1. ss. hexploit step_map; ss.
+        { eapply ident_map_le. }
+        { eapply ident_map_bot. }
+        { eapply ident_map_eq. }
+        { instantiate (1:=fun _ => True). i. eapply ident_map_mappable_evt. }
+        { econs; eauto. econs; eauto. }
+        { ss. }
+        { eauto. }
+        { ss. }
+        { ss. }
+        { ss. }
+        { eapply mapping_map_lt_collapsable_unwritable. eapply ident_map_lt. }
+        { ss. }
+        i. des. inv STEP0.
+        assert (RECHABLE0: semi_reachable (Thread.mk _ state flc1 fsc1 fmem1)).
+        { inv REACHABLE.
+          econs; eauto. etrans; eauto. econs 2; [|refl]. econs; eauto. econs; eauto.
+          ss. inv LOCAL1. hexploit promise_consistent_map.
+          { eapply ident_map_le. }
+          { eapply ident_map_eq. }
+          { eapply TVIEW. }
+          { eapply PROMISES. }
+          { ss. }
+          i. eapply promise_consistent_mon; eauto. refl.
+        }
+        esplits; eauto. econs; eauto.
+        { eapply mapping_map_lt_collapsable_unwritable; eauto. eapply ident_map_lt. }
+      Qed.
+
+      Lemma tau_steps_map_reachable lang (th0 th1 fth0: Thread.t lang)
+            (STEPS: rtc (@Thread.tau_step _) th0 th1)
+            (THREAD: thread_map ident_map th0 fth0)
+            (CONSISTENT: Local.promise_consistent th1.(Thread.local))
+            (REACHABLE: semi_reachable fth0)
+            (LOCAL: Local.wf th0.(Thread.local) th0.(Thread.memory))
+            (MEMORY: Memory.closed th0.(Thread.memory))
+            (SC: Memory.closed_timemap th0.(Thread.sc) th0.(Thread.memory))
+            (FLOCAL: Local.wf fth0.(Thread.local) fth0.(Thread.memory))
+            (FMEMORY: Memory.closed fth0.(Thread.memory))
+            (FSC: Memory.closed_timemap fth0.(Thread.sc) fth0.(Thread.memory))
+        :
+          exists fth1,
+            (<<STEPS: rtc (@Thread.tau_step _) fth0 fth1>>) /\
+            (<<THREAD: thread_map ident_map th1 fth1>>) /\
+            (<<REACHABLE: semi_reachable fth1>>) /\
+            (<<STEPS: rtc (@tau_step _) th0 th1>>)
+      .
+      Proof.
+        revert_until STEPS. revert fth0. induction STEPS; eauto.
+        { i. esplits; eauto. }
+        i. inv H. inv TSTEP. exploit Thread.step_future; eauto. i. des.
+        hexploit PromiseConsistent.rtc_tau_step_promise_consistent; eauto. i.
+        hexploit step_map_reachable; eauto. i. des.
+        exploit Thread.step_future; try apply STEP0; eauto. i. des.
+        hexploit IHSTEPS; eauto. i. des. exists fth2. splits; auto.
+        { eapply tevent_map_same_machine_event in EVENT0.
+          rewrite <- EVENT0 in EVENT.
+          econs 2; eauto. econs; eauto. econs; eauto.
+        }
+        { econs 2; eauto. econs; eauto. }
+      Qed.
+
+      Lemma consistent_reachable lang (th0: Thread.t lang)
+            (CONSISTENT: Thread.consistent th0)
+            (REACHABLE: semi_reachable th0)
+            (LOCAL: Local.wf th0.(Thread.local) th0.(Thread.memory))
+            (MEMORY: Memory.closed th0.(Thread.memory))
+            (SC: Memory.closed_timemap th0.(Thread.sc) th0.(Thread.memory))
+        :
+          consistent th0.
+      Proof.
+        ii.
+        assert (THREAD: thread_map ident_map (Thread.mk _ th0.(Thread.state) th0.(Thread.local) sc1 mem1) th0).
+        { destruct th0. ss. econs; eauto.
+          - eapply ident_map_local.
+          - econs.
+            + i. eapply Memory.cap_inv in GET; eauto. des; eauto.
+              right. exists to, from, msg, msg. splits; ss.
+              * eapply ident_map_message.
+              * refl.
+            + i. eapply Memory.cap_le in GET; eauto; [|refl].
+              left. exists fto, ffrom, fto, ffrom. splits; ss; try refl. i. econs; eauto.
+          - eapply mapping_map_lt_collapsable_unwritable. eapply ident_map_lt.
+          - eapply ident_map_timemap.
+          - eapply Memory.max_concrete_timemap_spec; eauto.
+            eapply Memory.cap_closed_timemap; eauto.
+        }
+        assert (FLOCAL: Local.wf th0.(Thread.local) mem1).
+        { eapply Local.cap_wf; eauto. }
+        assert (FMEMORY: Memory.closed mem1).
+        { eapply Memory.cap_closed; eauto. }
+        assert (FSC: Memory.closed_timemap sc1 mem1).
+        { eapply Memory.max_concrete_timemap_closed; eauto. }
+        exploit CONSISTENT; eauto. i. des.
+        { left. unfold Thread.steps_failure in *. des.
+          exploit Thread.rtc_tau_step_future; eauto. i. des. ss.
+          eapply tau_steps_map_reachable in STEPS; eauto.
+          { des. exploit Thread.rtc_tau_step_future; eauto. i. des.
+            eapply step_map_reachable in FAILURE0; eauto.
+            { des. esplits; eauto. }
+            { inv FAILURE0; inv STEP. inv LOCAL0. inv LOCAL1. ss. }
+          }
+          { inv FAILURE0; inv STEP. inv LOCAL0. inv LOCAL1. ss. }
+        }
+        { right. eapply tau_steps_map_reachable in STEPS; eauto.
+          { des. esplits; eauto. }
+          { eapply Local.bot_promise_consistent; eauto. }
+        }
+      Qed.
+
+      Lemma configuration_step_reachable c1 c2 e
+            (STEP: SConfiguration.step e tid c1 c2)
+            (REACHABLE: rtc SConfiguration.all_machine_step c0 c1)
+            (WF: Configuration.wf c1)
+        :
+          configuration_step e tid c1 c2.
+      Proof.
+        inv STEP.
+        exploit Thread.rtc_cancel_step_future; eauto; try eapply WF; eauto. i. des. ss.
+        exploit Thread.opt_step_future; eauto. i. des.
+        exploit Thread.rtc_reserve_step_future; eauto. i. des. ss.
+        assert ((<<CONSISTENT4: Local.promise_consistent lc4>>) /\
+                (<<CONSISTENT3: Local.promise_consistent e3.(Thread.local)>>)).
+        { destruct (classic (e = ThreadEvent.failure)).
+          - subst. inv STEP0. inv STEP; inv STEP0. inv LOCAL. inv LOCAL0. ss.
+            splits; eauto.
+            eapply PromiseConsistent.rtc_reserve_step_promise_consistent2 in RESERVES; eauto.
+          - specialize (CONSISTENT H).
+            eapply PromiseConsistent.consistent_promise_consistent in CONSISTENT; eauto.
+            splits; eauto.
+            eapply PromiseConsistent.rtc_reserve_step_promise_consistent; eauto.
+        }
+        des.
+        assert (CONSISTENT2: Local.promise_consistent e2.(Thread.local)).
+        { inv STEP0; eauto.
+          eapply PromiseConsistent.step_promise_consistent; eauto. }
+        assert (CONSISTENT1: Local.promise_consistent lc1).
+        { eapply PromiseConsistent.rtc_cancel_step_promise_consistent in CANCELS; eauto. }
+        eapply cancel_steps_reachable in CANCELS; eauto; try eapply WF; eauto. des.
+        eapply opt_step_reachable in STEP0; eauto. des.
+        eapply reserve_steps_reachable in RESERVES; eauto. des.
+        econs; eauto. i.
+        eapply consistent_reachable; eauto.
+      Qed.
+
+    End TID.
+
+    Section SIMCONFIG.
+
+      Inductive sim_state_rel
+                (tid: Ident.t)
+                (lang_src lang_tgt: language)
+                (r: Language.state lang_src -> Language.state lang_tgt -> Prop) :=
+      | sim_state_rel_intro
+          (STEP: forall st_src0 st_tgt0 st_tgt1 e
+                        (REL: r st_src0 st_tgt0)
+                        (REACHABLE: semi_reachable_state tid lang_tgt st_tgt1)
+                        (STEP: Language.step lang_tgt e st_tgt0 st_tgt1),
+              exists st_src1,
+                (<<STEP: Language.step lang_src e st_src0 st_src1>>) /\
+                (<<REL: r st_src1 st_tgt1>>))
+          (TERMINAL: forall st_src st_tgt
+                            (REL: r st_src st_tgt)
+                            (REACHABLE: semi_reachable_state tid lang_tgt st_tgt)
+                            (TERMINAL: Language.is_terminal lang_tgt st_tgt),
+              Language.is_terminal lang_src st_src)
+      .
+      Hint Constructors sim_state_rel.
+
+      Lemma eq_sim_state_rel tid lang
+        :
+          sim_state_rel tid lang lang eq.
+      Proof.
+        econs; i; clarify. eauto.
+      Qed.
+
+      Variable (r: forall (tid: Ident.t) (lang_src lang_tgt: language),
+                   Language.state lang_src -> Language.state lang_tgt -> Prop).
+      Hypothesis (REL: forall tid lang_src lang_tgt, sim_state_rel tid lang_src lang_tgt (r tid lang_src lang_tgt)).
+
+      Inductive sim_statelocal tid:
+        forall (lcst_src lcst_tgt: (sigT (@Language.state _)) * Local.t), Prop :=
+      | sim_statelocal_intro
+          lang_src lang_tgt st_src st_tgt lc
+          (REL: r tid lang_src lang_tgt st_src st_tgt)
+        :
+          sim_statelocal tid (existT _ lang_src st_src, lc) (existT _ lang_tgt st_tgt, lc)
+      .
+      Hint Constructors sim_statelocal.
+
+      Inductive sim_thread tid lang_src lang_tgt: forall (th_src: Thread.t lang_src) (th_tgt: Thread.t lang_tgt), Prop :=
+      | sim_thread_intro
+          st_src st_tgt lc sc mem
+          (REL: r tid lang_src lang_tgt st_src st_tgt)
+        :
+          sim_thread tid (Thread.mk _ st_src lc sc mem) (Thread.mk _ st_tgt lc sc mem)
+      .
+      Hint Constructors sim_thread.
+
+      Inductive sim_configuration:
+        forall (c_src c_tgt: Configuration.t), Prop :=
+      | sim_configuration_intro
+          ths_src ths_tgt sc mem
+          (THS: forall tid,
+              option_rel
+                (sim_statelocal tid)
+                (IdentMap.find tid ths_src)
+                (IdentMap.find tid ths_tgt))
+        :
+          sim_configuration (Configuration.mk ths_src sc mem) (Configuration.mk ths_tgt sc mem)
+      .
+      Hint Constructors sim_configuration.
+
+      Lemma sim_thread_step tid lang_src lang_tgt
+            (th_src0: Thread.t lang_src) (th_tgt0 th_tgt1: Thread.t lang_tgt) pf e
+            (STEP: step tid pf e th_tgt0 th_tgt1)
+            (SIM: sim_thread tid th_src0 th_tgt0)
+        :
+          exists th_src1,
+            (<<STEP: Thread.step pf e th_src0 th_src1>>) /\
+            (<<SIM: sim_thread tid th_src1 th_tgt1>>).
+      Proof.
+        inv SIM. inv STEP; ss. inv STEP0.
+        { inv STEP. ss. esplits; eauto. econs 1; eauto. econs; eauto. }
+        inv STEP. specialize (REL tid lang_src lang_tgt). inv REL.
+        exploit STEP; eauto. i. des.
+        esplits; eauto.
+      Qed.
+
+      Lemma sim_thread_opt_step tid lang_src lang_tgt
+            (th_src0: Thread.t lang_src) (th_tgt0 th_tgt1: Thread.t lang_tgt) e
+            (STEP: opt_step tid e th_tgt0 th_tgt1)
+            (SIM: sim_thread tid th_src0 th_tgt0)
+        :
+          exists th_src1,
+            (<<STEP: Thread.opt_step e th_src0 th_src1>>) /\
+            (<<SIM: sim_thread tid th_src1 th_tgt1>>).
+      Proof.
+        inv STEP.
+        - esplits; eauto. econs 1.
+        - eapply sim_thread_step in SIM; eauto. des. esplits; eauto. econs 2; eauto.
+      Qed.
+
+      Lemma sim_thread_reserve_steps tid lang_src lang_tgt
+            (th_src0: Thread.t lang_src) (th_tgt0 th_tgt1: Thread.t lang_tgt)
+            (STEPS: rtc (@reserve_step tid _) th_tgt0 th_tgt1)
+            (SIM: sim_thread tid th_src0 th_tgt0)
+        :
+          exists th_src1,
+            (<<STEPS: rtc (@Thread.reserve_step _) th_src0 th_src1>>) /\
+            (<<SIM: sim_thread tid th_src1 th_tgt1>>).
+      Proof.
+        ginduction STEPS; eauto. i. inv H.
+        eapply sim_thread_step in STEP; eauto. des.
+        exploit IHSTEPS; eauto. i. des.
+        exists th_src2; eauto. esplits; eauto. econs; eauto. econs; eauto.
+      Qed.
+
+      Lemma sim_thread_cancel_steps tid lang_src lang_tgt
+            (th_src0: Thread.t lang_src) (th_tgt0 th_tgt1: Thread.t lang_tgt)
+            (STEPS: rtc (@cancel_step tid _) th_tgt0 th_tgt1)
+            (SIM: sim_thread tid th_src0 th_tgt0)
+        :
+          exists th_src1,
+            (<<STEPS: rtc (@Thread.cancel_step _) th_src0 th_src1>>) /\
+            (<<SIM: sim_thread tid th_src1 th_tgt1>>).
+      Proof.
+        ginduction STEPS; eauto. i. inv H.
+        eapply sim_thread_step in STEP; eauto. des.
+        exploit IHSTEPS; eauto. i. des.
+        exists th_src2; eauto. esplits; eauto. econs; eauto. econs; eauto.
+      Qed.
+
+      Lemma sim_thread_tau_steps tid lang_src lang_tgt
+            (th_src0: Thread.t lang_src) (th_tgt0 th_tgt1: Thread.t lang_tgt)
+            (STEPS: rtc (@tau_step tid _) th_tgt0 th_tgt1)
+            (SIM: sim_thread tid th_src0 th_tgt0)
+        :
+          exists th_src1,
+            (<<STEPS: rtc (@Thread.tau_step _) th_src0 th_src1>>) /\
+            (<<SIM: sim_thread tid th_src1 th_tgt1>>).
+      Proof.
+        ginduction STEPS; eauto. i. inv H. inv TSTEP.
+        eapply sim_thread_step in STEP; eauto. des.
+        exploit IHSTEPS; eauto. i. des.
+        exists th_src2; eauto. esplits; eauto. econs; eauto. econs; eauto. econs; eauto.
+      Qed.
+
+      Lemma sim_thread_consistent tid lang_src lang_tgt
+            (th_src: Thread.t lang_src) (th_tgt: Thread.t lang_tgt)
+            (CONSISTENT: consistent tid th_tgt)
+            (SIM: sim_thread tid th_src th_tgt)
+        :
+          Thread.consistent th_src.
+      Proof.
+        inv SIM. ii; ss.
+        assert (SIM: sim_thread tid (Thread.mk _ st_src lc sc1 mem1) (Thread.mk _ st_tgt lc sc1 mem1)).
+        { econs; eauto. }
+        exploit CONSISTENT; eauto. i; ss. des.
+        - left. eapply sim_thread_tau_steps in STEPS; eauto. des.
+          eapply sim_thread_step in FAILURE; eauto. des.
+          unfold Thread.steps_failure. esplits; eauto.
+        - right. eapply sim_thread_tau_steps in STEPS; eauto. des.
+          esplits; eauto. inv SIM0. ss.
+      Qed.
+
+      Lemma sim_configuration_step c_src0 c_tgt0 c_tgt1 e tid
+            (WF: Configuration.wf c_tgt0)
+            (STEP: SConfiguration.step e tid c_tgt0 c_tgt1)
+            (SIM: sim_configuration c_src0 c_tgt0)
+            (REACHABLE: rtc SConfiguration.all_machine_step c0 c_tgt0)
+        :
+          exists c_src1,
+            (<<STEP: SConfiguration.step e tid c_src0 c_src1>>) /\
+            (<<SIM: sim_configuration c_src1 c_tgt1>>).
+      Proof.
+        eapply configuration_step_reachable in STEP; eauto.
+        inv STEP. inv SIM. ss.
+        dup THS. specialize (THS0 tid). setoid_rewrite TID in THS0.
+        unfold option_rel in THS0. des_ifs. destruct p as [[lang_src st_src] lc_tgt].
+        inv THS0. eapply inj_pair2 in H4. clarify. eapply inj_pair2 in H0. clarify.
+        assert (SIM: sim_thread tid (Thread.mk _ st_src lc1 sc mem) (Thread.mk _ st1 lc1 sc mem)) by eauto.
+        eapply sim_thread_cancel_steps in CANCELS; eauto. des.
+        eapply sim_thread_opt_step in STEP0; eauto. des.
+        eapply sim_thread_reserve_steps in RESERVES; eauto. des. destruct th_src2.
+        esplits.
+        { econs; s.
+          - eauto.
+          - eapply STEPS.
+          - eapply STEP.
+          - eapply STEPS0.
+          - i. eapply sim_thread_consistent; eauto.
+        }
+        { inv SIM2. ss. econs; eauto. i.
+          repeat erewrite IdentMap.gsspec. des_ifs.
+        }
+      Qed.
+
+      Lemma steps_configuration_local_consistent c1
+            (REACHABLE: rtc SConfiguration.all_machine_step c0 c1)
+            tid lang st lc
+            (TID: IdentMap.find tid c1.(Configuration.threads) = Some (existT _ lang st, lc))
+        :
+          Local.promise_consistent lc.
+      Proof.
+        eapply Operators_Properties.clos_rt_rt1n_iff in REACHABLE.
+        eapply Operators_Properties.clos_rt_rtn1_iff in REACHABLE.
+        revert tid lang st lc TID. induction REACHABLE; eauto.
+        i. inv H. inv STEP. assert (WF0: Configuration.wf y).
+        { eapply Operators_Properties.clos_rt_rtn1_iff in REACHABLE.
+          eapply Operators_Properties.clos_rt_rt1n_iff in REACHABLE.
+          eapply SConfiguration.all_machine_steps_future; eauto. }
+        exploit SConfiguration.step_future; eauto. i. des.
+        inv STEP0. ss.
+        erewrite IdentMap.gsspec in TID. des_ifs.
+        { eapply inj_pair2 in H0. clarify.
+          destruct (classic (e0 = ThreadEvent.failure)).
+          { inv STEP; ss. inv STEP0; inv STEP. inv LOCAL. inv LOCAL0.
+            eapply PromiseConsistent.rtc_reserve_step_promise_consistent2 in RESERVES; eauto.
+          }
+          { hexploit PromiseConsistent.consistent_promise_consistent; eauto; try apply WF2; eauto.
+            ss. inv WF2. ss. eapply WF; eauto.
+            erewrite IdentMap.gss. eauto.
+          }
+        }
+        { eapply IHREACHABLE; eauto. }
+      Qed.
+
+      Lemma sim_configuration_terminal c_src c_tgt
+            (TERMINAL: Configuration.is_terminal c_tgt)
+            (SIM: sim_configuration c_src c_tgt)
+            (REACHABLE: rtc SConfiguration.all_machine_step c0 c_tgt)
+        :
+          Configuration.is_terminal c_src.
+      Proof.
+        ii. inv SIM. ss.
+        specialize (THS tid). setoid_rewrite FIND in THS.
+        unfold option_rel in THS. des_ifs. destruct p as [[lang_tgt st_tgt] lc_tgt].
+        inv THS. eapply inj_pair2 in H4. clarify. eapply inj_pair2 in H0. clarify.
+        exploit TERMINAL; eauto. i. des.
+        specialize (REL tid lang lang_tgt). inv REL.
+        exploit TERMINAL0; eauto.
+        econs; eauto. econs; eauto. ss.
+        hexploit steps_configuration_local_consistent.
+        { eapply REACHABLE. }
+        { ss. eauto. }
+        { eauto. }
+      Qed.
+
+      Lemma sim_configuration_behavior c_src c_tgt
+            (WF: Configuration.wf c_tgt)
+            (SIM: sim_configuration c_src c_tgt)
+            (REACHABLE: rtc SConfiguration.all_machine_step c0 c_tgt)
+        :
+          behaviors SConfiguration.machine_step c_tgt <1= behaviors SConfiguration.machine_step c_src.
+      Proof.
+        intros beh BEH. ginduction BEH; eauto.
+        - i. econs 1. eapply sim_configuration_terminal; eauto.
+        - i. dup STEP. inv STEP0. exploit SConfiguration.step_future; eauto. i. des.
+          eapply sim_configuration_step in STEP1; eauto. des. econs 2.
+          + rewrite <- H0. econs; eauto.
+          + eapply IHBEH; eauto. etrans; eauto.
+        - i. dup STEP. inv STEP0. exploit SConfiguration.step_future; eauto. i. des.
+          eapply sim_configuration_step in STEP1; eauto. des. econs 3.
+          + rewrite <- H0. econs; eauto.
+        - i. dup STEP. inv STEP0. exploit SConfiguration.step_future; eauto. i. des.
+          eapply sim_configuration_step in STEP1; eauto. des. econs 4.
+          + rewrite <- H0. econs; eauto.
+          + eapply IHBEH; eauto. etrans; eauto.
+      Qed.
+    End SIMCONFIG.
+  End REACHABLE.
+
+  Theorem unreachable_code_transformation syn_src syn_tgt
+          (r: forall (tid: Ident.t) (lang_src lang_tgt: language),
+              Language.state lang_src -> Language.state lang_tgt -> Prop)
+          (REL: forall tid lang_src lang_tgt, sim_state_rel (Configuration.init syn_tgt) tid lang_src lang_tgt (r tid lang_src lang_tgt))
+          (INIT: sim_configuration r (Configuration.init syn_src) (Configuration.init syn_tgt))
+    :
+      behaviors SConfiguration.machine_step (Configuration.init syn_tgt)
+      <1=
+      behaviors SConfiguration.machine_step (Configuration.init syn_src).
+  Proof.
+    eapply sim_configuration_behavior; eauto.
+    - i. ss. unfold Threads.init in *. rewrite IdentMap.Facts.map_o in TID.
+      unfold option_map in *. des_ifs. ii. ss. erewrite Memory.bot_get in *. ss.
+    - eapply Configuration.init_wf.
+    - eapply Configuration.init_wf.
+  Qed.
+End SemiReachable.
